refactor state machine safety

raft/StateMachineSafetyInterface.v
@@ -20,14 +20,6 @@ Section StateMachineSafety.
       eIndex e = eIndex e' ->
       e = e'.
 
-  Definition maxIndex_lastApplied net :=
-    forall h,
-      lastApplied (nwState net h) <= maxIndex (log (nwState net h)).
-
-  Definition maxIndex_commitIndex net :=
-    forall h,
-      commitIndex (nwState net h) <= maxIndex (log (nwState net h)).
-  
   Definition state_machine_safety_nw net :=
     forall h p t leaderId prevLogIndex prevLogTerm entries leaderCommit e,
       In p (nwPackets net) ->
@@ -39,8 +31,7 @@ Section StateMachineSafety.
        In e entries).
 
   Definition state_machine_safety net :=
-    state_machine_safety_host net /\ state_machine_safety_nw net /\
-    maxIndex_lastApplied net /\ maxIndex_commitIndex net.
+    state_machine_safety_host net /\ state_machine_safety_nw net.
 
   Class state_machine_safety_interface : Prop :=
     {
