raft/proof/StateMachineSafetyProof.v
@@ -123,70 +123,6 @@ Section StateMachineSafetyProof.
       end; intuition.
   Qed.
       
-  Lemma state_machine_safety_init :
-    refined_raft_net_invariant_init lifted_state_machine_safety.
-  Admitted.
-
-  Lemma state_machine_safety_client_request :
-    refined_raft_net_invariant_client_request lifted_state_machine_safety.
-  Admitted.
-
-  Lemma state_machine_safety_timeout :
-    refined_raft_net_invariant_timeout lifted_state_machine_safety.
-  Admitted.
-
-  Lemma state_machine_safety_append_entries :
-    refined_raft_net_invariant_append_entries lifted_state_machine_safety.
-  Admitted.
-
-  Lemma state_machine_safety_append_entries_reply :
-    refined_raft_net_invariant_append_entries_reply lifted_state_machine_safety.
-  Admitted.
-
-  Lemma state_machine_safety_request_vote :
-    refined_raft_net_invariant_request_vote lifted_state_machine_safety.
-  Admitted.
-
-  Lemma state_machine_safety_request_vote_reply :
-    refined_raft_net_invariant_request_vote_reply lifted_state_machine_safety.
-  Admitted.
-
-  Lemma state_machine_safety_do_leader :
-    refined_raft_net_invariant_do_leader lifted_state_machine_safety.
-  Admitted.
-
-  Lemma state_machine_safety_do_generic_server :
-    refined_raft_net_invariant_do_generic_server lifted_state_machine_safety.
-  Admitted.
-
-  Lemma state_machine_safety_state_same_packet_subset :
-    refined_raft_net_invariant_state_same_packet_subset lifted_state_machine_safety.
-  Admitted.
-
-  Lemma state_machine_safety_reboot :
-    refined_raft_net_invariant_reboot lifted_state_machine_safety.
-  Admitted.
-
-  Lemma state_machine_safety_invariant' :
-    forall net,
-      refined_raft_intermediate_reachable net ->
-      lifted_state_machine_safety net.
-  Proof.
-    intros.
-    apply refined_raft_net_invariant; auto.
-    - apply state_machine_safety_init.
-    - apply state_machine_safety_client_request.
-    - apply state_machine_safety_timeout.
-    - apply state_machine_safety_append_entries.
-    - apply state_machine_safety_append_entries_reply.
-    - apply state_machine_safety_request_vote.
-    - apply state_machine_safety_request_vote_reply.
-    - apply state_machine_safety_do_leader.
-    - apply state_machine_safety_do_generic_server.
-    - apply state_machine_safety_state_same_packet_subset.
-    - apply state_machine_safety_reboot.
-  Qed.
-
   Theorem state_machine_safety_invariant :
     forall net,
       raft_intermediate_reachable net ->
@@ -194,8 +130,9 @@ Section StateMachineSafetyProof.
   Proof.
     apply lower_prop.
     intros.
-    apply state_machine_safety_invariant' in H.
-    auto.
+    unfold state_machine_safety. split.
+    - auto using state_machine_safety_host_invariant.
+    - admit.
   Qed.
 
   Instance smsi : state_machine_safety_interface.
